rocq/theories/TypeSystem/TypeSafetyBasePreservationMutual.v
@@ -599,7 +599,7 @@ Proof.
   induction Htail as
     [lts args Σ branches expected_core
     |Σ branches v rest e0 T0 Σv_payload Σv Σs Ts expected_core
-       binders ps lts args Hfields_empty Hbinders_empty Hbinders Hparams
+       binders ps lts args Hbinders Hparams
        Hnodup Hctx_none Hlookup Htyped Hparams_ok Hremove Hcore
        Htail IHtail];
     intros Hvariant Hbranch.
@@ -622,18 +622,19 @@ Qed.
 Lemma typed_match_tail_lookup_no_payload :
   forall env Ω n lts args Σ branches variants expected_core Σs Ts
       name vdef binders,
+    preservation_ready_match_branches branches ->
     typed_match_tail_env_structural env Ω n lts args Σ branches variants
       expected_core Σs Ts ->
     lookup_enum_variant name variants = Some vdef ->
     lookup_expr_branch_binders name branches = Some binders ->
-    enum_variant_fields vdef = [] /\ binders = [].
+    binders = [].
 Proof.
   intros env Ω n lts args Σ branches variants expected_core Σs Ts
-    name vdef binders Htail.
+    name vdef binders Hready Htail.
   induction Htail as
     [lts args Σ branches expected_core
     |Σ branches v rest e0 T0 Σv_payload Σv Σs Ts expected_core
-       binders0 ps lts args Hfields_empty Hbinders_empty Hbinders
+       binders0 ps lts args Hbinders
        Hparams Hnodup Hctx_none Hlookup Htyped Hparams_ok Hremove Hcore
        Htail IHtail];
     intros Hvariant Hbranch_binders.
@@ -644,7 +645,8 @@ Proof.
       inversion Hvariant; subst vdef.
       rewrite Hbinders in Hbranch_binders.
       inversion Hbranch_binders; subst binders.
-      split; assumption.
+      eapply lookup_expr_branch_binders_preservation_ready_empty;
+        eassumption.
     + eapply IHtail; eassumption.
 Qed.
 
@@ -1407,25 +1409,27 @@ Proof.
         end.
 	      }
 	      subst e_branch.
-	      assert (Hfields_runtime : enum_variant_fields vdef_runtime = []).
-	      { assert (Hedef_same : edef_runtime = edef) by congruence.
-	        subst edef_runtime.
-	        rewrite H6 in Hlookup_variant_runtime. simpl in Hlookup_variant_runtime.
-	        rewrite String.eqb_refl in Hlookup_variant_runtime.
-	        inversion Hlookup_variant_runtime; subst. exact H7. }
+	      assert (Hbinders_head_nil : binders_head = []).
+	      { eapply lookup_expr_branch_binders_preservation_ready_empty;
+	          eassumption. }
 	      assert (Hbinders_nil : binders = []).
-	      { rewrite Hlookup_binders in H9. inversion H9. reflexivity. }
+	      { eapply lookup_expr_branch_binders_preservation_ready_empty;
+	          eassumption. }
 	      assert (Hpayload_nil : ps_payload = []).
 	      { unfold match_payload_params_opt in Hpayload_runtime.
 	        unfold TypingRules.match_payload_params_opt in Hpayload_runtime.
-	        rewrite Hfields_runtime in Hpayload_runtime.
 	        rewrite Hbinders_nil in Hpayload_runtime.
-	        simpl in Hpayload_runtime. inversion Hpayload_runtime. reflexivity. }
+	        destruct (enum_variant_fields vdef_runtime) as [| field fields];
+	          simpl in Hpayload_runtime; try discriminate.
+	        inversion Hpayload_runtime. reflexivity. }
 	      assert (Hps_head_nil : ps_head = []).
-	      { unfold match_payload_params in H10.
-	        unfold instantiate_enum_variant_field_tys in H10.
-	        rewrite H7 in H10. simpl in H10.
-	        inversion H10. reflexivity. }
+	      { unfold match_payload_params in H8.
+	        unfold instantiate_enum_variant_field_tys in H8.
+	        rewrite Hbinders_head_nil in H8.
+	        destruct (map (instantiate_enum_variant_field_ty lts args)
+	          (enum_variant_fields v_head)) as [| field fields];
+	          try discriminate.
+	        inversion H8. reflexivity. }
 	      assert (Hvalues_nil : values = []).
 	      { rewrite Hpayload_nil in Hvalues_len.
 	        destruct values as [| value values']; simpl in Hvalues_len;
@@ -1440,10 +1444,10 @@ Proof.
 	        as [Hstore_branch [Hv_branch Hpres_branch]].
 	      split.
 	      * subst s'. rewrite Hpayload_nil. simpl.
-	        rewrite Hps_head_nil in H17. simpl in H17.
+	        rewrite Hps_head_nil in H15. simpl in H15.
 	        eapply store_typed_ctx_merge_many_left.
 	        -- exact Hstore_branch.
-	        -- exact H17.
+	        -- exact H15.
 	      * split.
 	        -- rewrite Hremove_params, Hpayload_nil. simpl.
 	           eapply value_has_type_match_head_result. exact Hv_branch.
@@ -1461,7 +1465,7 @@ Proof.
 	      subst vdef_typed_runtime.
 	      destruct (typed_match_tail_lookup env Ω n lts args Σ1 branches v_tail
 		            (ty_core T_head) Σ_tail Ts_tail variant_name vdef_runtime e_branch
-		            H16 Hvariant_runtime Hlookup_branch_eval)
+		            H14 Hvariant_runtime Hlookup_branch_eval)
 	          as [T_branch [Σ_branch_payload [Σ_branch [ps_branch
 	             [binders_branch Htail_branch]]]]];
 	      destruct Htail_branch as [Hbinders_branch Htail_branch].
@@ -1501,10 +1505,14 @@ Proof.
 	        - exact H0.
 	        - exact H1.
 	        - exact Hvariant_runtime_full. }
-	      destruct (typed_match_tail_lookup_no_payload env Ω n lts args Σ1
+	      pose proof (typed_match_tail_lookup_no_payload env Ω n lts args Σ1
 	          branches v_tail (ty_core T_head) Σ_tail Ts_tail
-	          variant_name vdef_runtime binders_branch H16 Hvariant_runtime
-	          Hbinders_branch) as [Hfields_runtime_tail Hbinders_branch_nil].
+	          variant_name vdef_runtime binders_branch
+	          ltac:(match goal with
+	            | Hready_branches : preservation_ready_match_branches branches |- _ =>
+	                exact Hready_branches
+	            end)
+	          H14 Hvariant_runtime Hbinders_branch) as Hbinders_branch_nil.
 	      assert (Hbinders_nil : binders = []).
 	      { rewrite Hbinders_branch_nil in Hbinders_branch.
 	        rewrite Hlookup_binders in Hbinders_branch.
@@ -1512,15 +1520,17 @@ Proof.
 	      assert (Hpayload_nil : ps_payload = []).
 	      { unfold match_payload_params_opt in Hpayload_runtime.
 	        unfold TypingRules.match_payload_params_opt in Hpayload_runtime.
-	        rewrite Hfields_runtime_tail in Hpayload_runtime.
 	        rewrite Hbinders_nil in Hpayload_runtime.
-	        simpl in Hpayload_runtime. inversion Hpayload_runtime. reflexivity. }
+	        destruct (enum_variant_fields vdef_runtime) as [| field fields];
+	          simpl in Hpayload_runtime; try discriminate.
+	        inversion Hpayload_runtime. reflexivity. }
 	      assert (Hps_branch_nil : ps_branch = []).
 	      { unfold match_payload_params_opt in Hparams_branch.
 	        unfold TypingRules.match_payload_params_opt in Hparams_branch.
-	        rewrite Hfields_runtime_tail in Hparams_branch.
 	        rewrite Hbinders_branch_nil in Hparams_branch.
-	        simpl in Hparams_branch. inversion Hparams_branch. reflexivity. }
+	        destruct (enum_variant_fields vdef_runtime) as [| field fields];
+	          simpl in Hparams_branch; try discriminate.
+	        inversion Hparams_branch. reflexivity. }
 	      assert (Hvalues_nil : values = []).
 	      { rewrite Hpayload_nil in Hvalues_len.
 	        destruct values as [| value values']; simpl in Hvalues_len;
@@ -1538,13 +1548,19 @@ Proof.
 	      destruct (IHbranch Ω n (sctx_add_params ps_branch Σ1) T_branch
 	                  Σ_branch_payload Hready_branch Hstore_payload Htyped_branch)
 	        as [Hstore_branch [Hv_branch Hpres_branch]].
+	      assert (Hbinders_head_nil_tail : binders_head = []).
+	      { eapply lookup_expr_branch_binders_preservation_ready_empty;
+	          eassumption. }
 	      assert (Hps_head_nil_tail : ps_head = []).
-	      { unfold match_payload_params in H10.
-	        unfold instantiate_enum_variant_field_tys in H10.
-	        rewrite H7 in H10. simpl in H10.
-	        inversion H10. reflexivity. }
+	      { unfold match_payload_params in H8.
+	        unfold instantiate_enum_variant_field_tys in H8.
+	        rewrite Hbinders_head_nil_tail in H8.
+	        destruct (map (instantiate_enum_variant_field_ty lts args)
+	          (enum_variant_fields v_head)) as [| field fields];
+	          try discriminate.
+	        inversion H8. reflexivity. }
 	      pose (Σ_head := sctx_remove_params ps_head Σ_head_payload).
-	      fold Σ_head in H17.
+	      fold Σ_head in H15.
 	      assert (Hsame_head_tail : Forall (sctx_same_bindings Σ_head) Σ_tail).
 	      {
 	        assert (Hsame_head : sctx_same_bindings Σ1 Σ_head).
